concurrency/hack-hash-table/ResourceStateMachine.i.dfy
@@ -1,0 +1,44 @@
+include "HTResource.i.dfy"
+
+module ResourceStateMachine {
+  import opened KeyValueType
+
+  import HT = HTResource
+  import MapIfc
+
+  type Variables = HT.R
+
+  predicate Init(s: Variables)
+  {
+    HT.Init(s)
+  }
+
+  predicate Internal(s: Variables, s': Variables)
+  {
+    HT.Update(s, s')
+  }
+
+  predicate NewTicket(s: Variables, s': Variables, id: int, input: MapIfc.Input)
+  {
+    s' == HT.add(s, HT.input_ticket(input))
+  }
+
+  predicate ConsumeStub(s: Variables, s': Variables, id: int, output: MapIfc.Input)
+  {
+    s == HT.add(s', HT.output_stub(output))
+  }
+
+  ////// Invariant
+
+  predicate Complete(s: Variables)
+  {
+    && (forall i | 0 <= i < |s.table| :: s.table[i].Some?)
+  }
+
+  predicate Inv(s: Variables)
+  {
+    && s.R?
+    && Complete(s)
+    && 
+  }
+}
